src/Assembly/Equivalence.v
@@ -44,7 +44,7 @@ Definition default_assembly_labels_fuzzy_prefixes : assembly_labels_fuzzy_prefix
 Class assembly_calling_registers_opt := assembly_calling_registers' : option (list REG).
 #[global]
 Typeclasses Opaque assembly_calling_registers_opt.
-Definition default_assembly_calling_registers := List.map ScalarReg [rdi;rsi;rdx;rcx;r8;r9].
+Definition default_assembly_calling_registers := List.map SReg [rdi;rsi;rdx;rcx;r8;r9].
 
 Definition assembly_calling_registers {v : assembly_calling_registers_opt} : list REG
   := Option.value v default_assembly_calling_registers.
@@ -58,12 +58,12 @@ The registers RBX, RBP, RDI, RSI, RSP, R12, R13, R14, and R15 are considered non
 
 -----
 [22] https://docs.microsoft.com/en-us/cpp/build/x64-calling-convention?view=msvc-170&viewFallbackFrom=vs-2019#callercallee-saved-registers *)
-Definition microsoft_x64_assembly_callee_saved_registers := List.map ScalarReg [rbx;rbp;rdi;rsi;rsp;r12;r13;r14;r15].
+Definition microsoft_x64_assembly_callee_saved_registers := List.map SReg [rbx;rbp;rdi;rsi;rsp;r12;r13;r14;r15].
 (* https://en.wikipedia.org/wiki/X86_calling_conventions#System_V_AMD64_ABI *)
 (* If the callee wishes to use registers RBX, RSP, RBP, and R12–R15, it must restore their original values before returning control to the caller. All other registers must be saved by the caller if it wishes to preserve their values.[25]: 16
 
 [25] Michael Matz; Jan Hubička; Andreas Jaeger; et al., eds. (2018-01-28). "System V Application Binary Interface: AMD64 Architecture Processor Supplement (With LP64 and ILP32 Programming Models) Version 1.0" (PDF). 1.0. https://github.com/hjl-tools/x86-psABI/wiki/x86-64-psABI-1.0.pdf *)
-Definition system_v_amd64_assembly_callee_saved_registers := List.map ScalarReg [rbx;rsp;rbp;r12;r13;r14;r15].
+Definition system_v_amd64_assembly_callee_saved_registers := List.map SReg [rbx;rsp;rbp;r12;r13;r14;r15].
 Definition default_assembly_callee_saved_registers := System_V_AMD64.
 Definition assembly_callee_saved_registers {v : assembly_callee_saved_registers_opt} : list REG
   := match v with
